split out AssocList

examples/FiniteMap.v
@@ -1,168 +1,29 @@
-(* This file defines a module interface for finite maps and two implementations,
- * one based on a ref to an association list, and one based on a hash-table.
- * The hash-table functor is parameterized by another finite map implementation
- * so that each bucket in the hash-table is implemented by a "nested" finite map.
- *)
+(* This file defines the interface for an imperative FiniteMap, which
+   is modeled by a function association list *)
 
 Require Import Ynot.
+Require Export AssocListModel.
+
 Set Implicit Arguments.
-(* Require Import Relations. *)
 
-(*************************************************)
-(* Module parameter for the finite map interface *)
-(*************************************************)
-Module Type ASSOCIATION.
-  Variable key_t : Set.
-  Variable value_t : key_t -> Set.  (* note that value types depend on the keys *)
-  Variable key_eq_dec : forall (k1 k2:key_t), {k1 = k2} + {k1 <> k2}.
-  Notation "k1 =! k2" := (key_eq_dec k1 k2) (at level 70, right associativity).
-End ASSOCIATION.
-
-(*********************************************)
-(* The functional model -- association lists *)
-(*********************************************)
-Module AssocList(A : ASSOCIATION).
-Require Export List.
-  Import A.
-  Notation "( x ,, y )" := (@existT _ _ x y) : core_scope.
-  Notation "` x" := (projT1 x) (at level 10): core_scope.
-
-  Require Import Eqdep_dec.
-  Module DecKey : DecidableType with Definition U:=A.key_t with Definition eq_dec:=A.key_eq_dec. 
-    Definition U := A.key_t.
-    Definition eq_dec := A.key_eq_dec.
-  End DecKey.
-  Module DecKeyFacts := DecidableEqDep(DecKey).
-
-  Definition key_eq_irr : (forall (k:A.key_t)(p:k = k), p = refl_equal k) := DecKeyFacts.UIP_refl.
-
-  (* because of the dependency of values on keys, we don't just use normal lists *)
-  Definition alist_t := list (sigT A.value_t).
-
-  Definition nil_al := @nil (sigT A.value_t).
-  Fixpoint remove(k:A.key_t)(l:alist_t) {struct l} : alist_t := 
-    match l with
-    | nil => nil
-    | (k',, v')::l' => if k =! k' then remove k l'
-                          else (k',, v')::(remove k l')
-    end.
-
-  Definition insert(k:A.key_t)(v:A.value_t k)(l:alist_t) := (k,, v)::(remove k l).
-
-  Definition coerce(k1 k2:A.key_t)(H:k1 = k2)(v:A.value_t k1) : A.value_t k2.
-    intros. rewrite H in v. apply v.
-  Defined.
-
-  Fixpoint lookup(k:A.key_t)(l:alist_t) {struct l} : option(A.value_t k) := 
-    match l with
-    | nil => None
-    | (k',, v'):: l' => 
-      match k' =! k with
-      | left k_eq_k' => Some (coerce k_eq_k' v')
-      | right k_neq_k' => lookup k l'
-      end
-    end.
-
-    Fixpoint distinct (l:alist_t) : Prop :=
-      match l with
-        | nil => True
-        | (k,,v)::ls => lookup k ls = None /\ distinct ls
-      end.
-    
-    Ltac simpler :=
-      repeat (progress ((repeat 
-        match goal with
-        | [H:?e = ?e |- _] => clear H
-        | [H:?k = ?k |- _ ] =>
-          match goal with
-            [|- context [H]] =>  rewrite (key_eq_irr H); simpl
-          end
-        | [|- context [match ?k1 =! ?k2 with 
-                         | left _ => _ 
-                         | right _ => _ end]] =>
-        case_eq (k1 =! k2) ; intros; try congruence ; try solve [assert False; intuition]; try subst 
-        | [H:context [match ?k1 =! ?k2 with 
-                         | left _ => _ 
-                         | right _ => _ end] |- _] =>
-        destruct (k1 =! k2) ; try congruence ; try solve [assert False; intuition]; try subst
-        |[H: sigT _ |- _] => destruct H
-        | [H: _ = _ |- context [coerce ?pf _]] => equate pf H || equate pf (sym_eq H)
-        | [H: _ = _ |- _ ] =>
-          match goal with
-            [|- context [H]] => let H2 := (fresh "H") in 
-              progress (generalize H; rewrite H; intro H2; rewrite (key_eq_irr H2); clear H2; simpl)
-          end
-        | [H: ?a = ?b |- _] => subst b || subst a
-      end); simpl in *; auto)).
-
-  (* interactions of lookup and the other operations *)
-  Lemma lookup_remove_eq k l : lookup k (remove k l) = None.
-  Proof. induction l; simpler. Qed.
-
-  Lemma lookup_remove_neq k k' l : k <> k' -> lookup k (remove k' l) = lookup k l.
-  Proof. induction l; simpler. Qed.
-
-  Lemma lookup_insert_eq k v l : lookup k (insert v l) = Some v.
-  Proof. induction l; simpler. Qed.
-
-  Lemma lookup_insert_neq k k' (v:value_t k') l : k <> k' -> lookup k (insert v l) = lookup k l.
-  Proof. induction l; simpler. Qed.
-
-  Lemma lookup_none_remove k l : lookup k l = None -> remove k l = l.
-  Proof. induction l; simpler. f_equal; auto. Qed.
-
-  Lemma lookup_none_perm k l l' : Permutation l l' -> lookup k l = None -> lookup k l' = None.
-  Proof. induction 1; simpler. Qed.
-
-  (* interactions of distinct and ther other operations *)
-  Lemma distinct_remove k l : distinct l -> distinct (remove k l).
-  Proof. induction l; simpler; intuition. rewrite lookup_remove_neq; auto. Qed.
-
-  Lemma distinct_insert k (v:A.value_t k) l : distinct l -> distinct (insert v l).
-  Proof. induction l; simpler; intuition. rewrite lookup_remove_neq; auto. Qed.
-
-  Lemma distinct_perm l l' : Permutation l l' -> distinct l -> distinct l'.
-  Proof. Hint Resolve lookup_none_perm. induction 1; simpler; intuition (congruence||eauto). Qed.
-
-  Hint Resolve lookup_remove_eq distinct_remove distinct_perm Permutation_sym Permutation_refl.
-
-  Lemma lookup_dis_perm k l l' : Permutation l l' -> distinct l -> lookup k l = lookup k l'.
-  Proof. induction 1; simpler; intuition try congruence. clear H1 H2; congruence. rewrite H2. eauto. Qed.
-
-  Lemma remove_perm k l l' : Permutation l l' -> Permutation (remove k l) (remove k l').
-  Proof.  Hint Constructors Permutation. induction 1; simpler; eauto. Qed.
-  Hint Resolve remove_perm.
-
-  Lemma insert_perm k l l' (v:A.value_t k) : Permutation l l' -> Permutation (insert v l) (insert v l').
-  Proof. unfold insert; simpler. Qed.
-  Hint Resolve insert_perm.
-
-  Lemma remove_swap k k' l : remove k (remove k' l) = remove k' (remove k l).
-  Proof. induction l; simpler. Qed.
-  Hint Resolve remove_swap.
-
-  Lemma insert_swap k (v:A.value_t k) k' (v':A.value_t k') l : k <> k' -> 
-    Permutation (insert v (insert v' l)) (insert v' (insert v l)).
-  Proof. intros. Hint Constructors Permutation. unfold insert; simpler. rewrite remove_swap. auto. Qed.
-  Hint Resolve insert_swap.
-
-End AssocList.
+(*********************************************************************************)
+(* This defines the type of the abstract object and its representation invariant *)
+(*********************************************************************************)
 
 Module Type FINITE_MAP_AT.
   Declare Module A:ASSOCIATION.
   Module AL := AssocList(A).
 
-  (* the abstract type of finite maps *)
+  (* The finite map's implementation's type *)
   Variable fmap_t : Set.
 
-  (* the abstract representation predicate -- connects an fmap_t to our model,
-   * which is an association list of (key,value) pairs. *)
+  (* Its representation invariant: relates an object and a functional model in a given heap *)
   Variable rep : fmap_t -> AL.alist_t -> hprop.
 End FINITE_MAP_AT.
 
-(*******************************************************************)
-(* The finite-map interface, relative to an ASSOCIATION definition *)
-(*******************************************************************)
+(*********************************************************************************************)
+(* The types of the finite map operations, relative to its implementation type and invariant *)
+(*********************************************************************************************)
 Module FINITE_MAP_T(Assoc:ASSOCIATION)(AT:FINITE_MAP_AT with Module A:=Assoc).
   Module A := AT.A.
   Module AL := AT.AL.
@@ -171,71 +32,43 @@ Module FINITE_MAP_T(Assoc:ASSOCIATION)(AT:FINITE_MAP_AT with Module A:=Assoc).
 
   Open Local Scope hprop_scope.
 
-  (* new returns an fmap_t that represents the empty association list *)
+  (* Allocates a new finite map *)
   Definition new := 
     STsep __ (fun (ans:fmap_t) => rep ans nil_al).
 
-  (* free takes an fmap_t that represents some association list, and destroys it *)
+  (* Frees a finite map *)
   Definition free := 
     forall (x:fmap_t)(l:[alist_t]), STsep (l ~~ rep x l) (fun (_:unit) => __).
 
-  (* insert takes an fmap_t that represents some association list l satisfying the
-   * predicate P, a key k, and a value v, and updates the fmap_t so it represents 
-   * (k,v)::l.  Note that, like the primitive ref-read construct in STsep, we have
-   * to use a predicate to characterize the model instead of universally quantifying
-   * over a computationally irrelevant version in order to get something useful -- 
-   * see the use in the hash-table below.
-   *)
+  (* Inserts a new key, value pair into the finite map. If the finite map already contains a
+     pair with the same key, it is overwritten *)
   Definition insert :=
     forall (x:fmap_t)(k:key_t)(v:value_t k)(l:[alist_t]),
       STsep (l ~~ rep x l)
         (fun (_:unit) => l ~~ rep x (insert v l)).
 
-  (* lookup takes an fmap_t that represents some list l satisfying the predicate P, 
-   * and a key k, and returns the value v associatied with k in l if any, while
-   * the map continues to represent l. *)
+  (* Returns Some(the value) corresponding to the given key in the finite map. 
+     Returns None if the key is not in the finite map *)
   Definition lookup :=
     forall (x:fmap_t)(k:key_t)(l:[alist_t]), 
       STsep (l ~~ rep x l) 
             (fun (ans:option (value_t k)) =>
                l ~~ [ans = lookup k l] * rep x l).
 
+  (* If the finite map contains a pair with the given key, it is
+     removed.  Otherwise, nothing happens. *)
   Definition remove :=
     forall (x:fmap_t)(k:key_t)(l:[alist_t]),
       STsep (l ~~ rep x l)
         (fun (_:unit) => l ~~ rep x (remove k l)).
 
-(*
-  Fixpoint fold_pre (B:Type) (P0:B->hprop)
-    (P:forall k, value_t k->B->hprop)
-    (Q:forall k, value_t k->B->B->hprop) (b:B)
-    (l:alist_t) {struct l}:=
-  match l with 
-    | nil => P0 b
-    | (k,,v)::ls => P k v b * [forall b', Q k v b b' ==> fold_pre P0 P Q b' ls]
-  end.
-
-  Fixpoint fold_post (B:Type) (Q0:B->hprop)
-    (Q:forall k, value_t k->B->B->hprop) (b:B) (ans:B)
-    (l:alist_t) {struct l}:=
-  match l with 
-    | nil => Q0 b * [b=ans]
-    | (k,,v)::ls => Exists b' :@ B, Q k v b b' & fold_post Q0 Q b' ans ls
-  end.
-
-  Definition hprop_forall T (p : T -> hprop) : hprop := fun h => forall v, p v h.
-  Notation "'Forall' v :@ T , p" := (hprop_forall (fun v : T => p)) (at level 90, T at next level) : hprop_scope.
-
-  Definition fold := forall (x:fmap_t)(B:Type) (P0:B->hprop) (P:forall k, value_t k->B->hprop) (Q0:B->hprop)
-                                               (Q:forall k, value_t k->B->B->hprop) (b:B)
-                                               (c:forall k v b, STsep (P k v b) (Q k v b)) (l:[alist_t]),
-    STsep (l ~~ rep x l * Forall l' :@ {l':alist_t | Permutation l l'}, fold_pre P0 P Q b (proj1_sig l'))
-    (fun (b':B) => (l ~~ rep x l * Exists l' :@ {l':alist_t | Permutation l l'}, fold_post Q0 Q b b' (proj1_sig l'))).
-*)
+  (* Models of finite maps do not have any duplicate keys. *)
   Definition distinct := forall (x:fmap_t) (l:alist_t), rep x l ==> [distinct l] * ??.
 
+  (* All permutations of a model are equally valid models of a finite map. *)
   Definition perm := forall (x:fmap_t) (l l':alist_t), Permutation l l' -> rep x l ==> rep x l'.
 
+  (* A simple tactic to unfold these types *)
   Ltac unfm_t := unfold new, free, insert, lookup, remove, distinct, perm.
 
 End FINITE_MAP_T.
@@ -244,7 +77,6 @@ End FINITE_MAP_T.
 (* The finite-map interface, relative to an ASSOCIATION definition *)
 (*******************************************************************)
 Module Type FINITE_MAP.
-(* do we need A? *)
   Declare Module A  : ASSOCIATION.
   Module AL := AssocList(A).
   Declare Module AT : FINITE_MAP_AT with Module A:=A with Module AL := AL.
@@ -257,108 +89,7 @@ Module Type FINITE_MAP.
   Parameter insert : T.insert.
   Parameter remove : T.remove.
   Parameter lookup : T.lookup.
-(*  Parameter fold : T.fold.  *)
   Axiom distinct : T.distinct.
   Axiom perm : T.perm.
 
 End FINITE_MAP.
-
-(*
-Module copier(FM:FINITE_MAP).
-Module AL := FM.AT.AL.
-Import AL.
-Import FM.
-
-Open Local Scope hprop_scope.
-Open Local Scope stsepi_scope.
-
-Fixpoint Tadd (sourceM destM:alist_t) {struct sourceM} :=
-  match sourceM with
-    | nil => destM
-    | (k,,v)::sourceM => AL.insert v (Tadd sourceM destM)
-  end.
-
-Lemma Tadd_perm1 l1 l1' l2 : Permutation l1 l1' -> AL.distinct l1 -> Permutation (Tadd l1 l2) (Tadd l1' l2).
-Proof. induction 1; simpler; intuition; try congruence. eapply perm_trans; eauto. Qed.
-
-Ltac simpl_inh := repeat 
-  match goal with
-    | [H:[_]%inhabited = [_]%inhabited |- _] => generalize (pack_injective H); clear H; intro H 
-    | [H1:?x = [?y1]%inhabited, H2:?x = [?y2]%inhabited |- _]
-      => match y1 with
-           | y2 => fail 1
-           | _ => rewrite H1 in H2
-         end
-  end.
-
-Lemma hprop_forall_conc T (P:T->hprop) Q : (forall x:T, Q ==> P x) -> Q ==> (T.hprop_forall P).
-Proof. firstorder. Qed.
-
-Ltac perm_simpl := 
-  match goal with
-  | [H:Permutation nil ?x |- _ ] => generalize (Permutation_nil H); clear H; intro H; subst x
-  | [H:Permutation ?x nil |- _ ] => generalize (Permutation_nil (Permutation_sym H)); clear H; intro H; subst x
-  | [H:Permutation (?a::?x1) ?x2 |- _ ] => 
-    match x2 with
-      | (_::_) => fail 1
-      | (_++_) => fail 1
-      | _ => destruct x2; [elim (Permutation_nil_cons (Permutation_sym H)) |]
-    end
-  | [H:Permutation ?x2 (?a::?x1) |- _ ] => 
-    match x2 with
-      | (_::_) => fail 1
-      | (_++_) => fail 1
-      | _ => destruct x2; [elim (Permutation_nil_cons H) |]
-    end
-end.
-(*
-Ltac simpler2 :=
-  repeat (progress ((repeat 
-    match goal with
-      | [H:[_]%inhabited = [_]%inhabited |- _] => generalize (pack_injective H); clear H; intro H 
-      | [H1:?x = [?y1]%inhabited, H2:?x = [?y2]%inhabited |- _]
-        => match y1 with
-             | y2 => fail 1
-             | _ => rewrite H1 in H2
-           end
-      | [|- context [match key_eq_dec ?k1 ?k2 with 
-                           | left _ => _ 
-                       | right _ => _ end]] =>
-      case_eq (key_eq_dec k1 k2) ; intros; try congruence ; try solve [assert False; intuition]; try subst
-        |[H: sigT _ |- _] => destruct H
-    end); simpl; auto)).
-*)
-
-Definition add (source ddest:fmap_t) (sourceM destM:[alist_t]) :
-  STsep (sourceM ~~ destM ~~ rep source sourceM * rep ddest destM)
-  (fun (_:unit) => sourceM ~~ destM ~~ rep source sourceM * rep ddest (Tadd sourceM destM)).
-intros.
-refine (zz <- (fold source _ _ _ _ destM (fun k v b => {{(insert ddest (k:=k) v b)}}
-                                         ;; {{Return (b ~~~ AL.insert v b)}}) sourceM)
-; {{Return tt}}); sep simpl_inh.
-assert (((fun (_:key_t) _ (x:[alist_t]) => (x ~~ rep ddest x)) k v [x]%inhabited) ==> rep ddest x); [idtac|eassumption].
-sep simpl_inh.
-assert (rep ddest (AL.insert v x0) ==> 
-   (fun _ _ l1 l2 => l2 ~~ rep ddest l2) k v [x0]%inhabited [AL.insert v x0]%inhabited); [idtac|eassumption].
-sep simpl_inh.
-apply hprop_forall_conc. destruct x1. simpl.
-revert x x0 p.
-induction x1; sep simpl_inh. 
-assert(rep ddest x ==> (fun x => x ~~ rep ddest x) [x]%inhabited); [sep simpl_inh|eassumption].
-destruct a.
-sep simpl_inh. repeat intro. destruct H. red. intuition. 
-sep auto.
-eapply IHx1. apply Permutation_refl.
-instantiate (1 := v). sep auto.
-instantiate (1 := v). sep auto.
-destruct v0. simpl.
-clear H2.
-revert x2 x1 p.
-induction x2; sep simpl_inh.
-perm_simpl. simpl.
-assert((fun x => x ~~ rep ddest x) [x]%inhabited ==> rep ddest x); [sep simpl_inh|eassumption].
-perm_simpl. simpler. sep auto. sep auto.
-pose (IHx2 ((_,,v)::x1)).
-change (rep ddest (Tadd ((_,,v0)::x1) x0) h).
-apply IHx1.
-*)
