examples/AssocListModel.v
@@ -1,0 +1,169 @@
+(* This files defines a module for an association type with a decidable equality on the keys
+  and an AssocList functor that provides a basic model of a functional association list based on
+  the provided association.  It is used as the model for FiniteMaps *)
+
+Require Import Ynot.
+Set Implicit Arguments.
+
+(*************************************************************************)
+(* Module that defines an association with decidable equality on the key *)
+(*************************************************************************)
+Module Type ASSOCIATION.
+  Variable key_t : Set.
+  Variable value_t : key_t -> Set.  (* note that value types depend on the keys *)
+  Variable key_eq_dec : forall (k1 k2:key_t), {k1 = k2} + {k1 <> k2}.
+  Notation "k1 =! k2" := (key_eq_dec k1 k2) (at level 70, right associativity).
+End ASSOCIATION.
+
+(*********************************************)
+(* The functional model -- association lists *)
+(*********************************************)
+Module AssocList(A : ASSOCIATION).
+Require Export List.
+  Import A.
+  Notation "( x ,, y )" := (@existT _ _ x y) : core_scope.
+  Notation "` x" := (projT1 x) (at level 10): core_scope.
+
+  Require Import Eqdep_dec.
+  Module DecKey : DecidableType with Definition U:=A.key_t with Definition eq_dec:=A.key_eq_dec. 
+    Definition U := A.key_t.
+    Definition eq_dec := A.key_eq_dec.
+  End DecKey.
+  Module DecKeyFacts := DecidableEqDep(DecKey).
+
+  Definition key_eq_irr : (forall (k:A.key_t)(p:k = k), p = refl_equal k) := DecKeyFacts.UIP_refl.
+
+  (* because of the dependency of values on keys, we don't just use normal lists *)
+  Definition alist_t := list (sigT A.value_t).
+
+  Definition nil_al := @nil (sigT A.value_t).
+  Fixpoint remove(k:A.key_t)(l:alist_t) {struct l} : alist_t := 
+    match l with
+    | nil => nil
+    | (k',, v')::l' => if k =! k' then remove k l'
+                          else (k',, v')::(remove k l')
+    end.
+
+  Definition insert(k:A.key_t)(v:A.value_t k)(l:alist_t) := (k,, v)::(remove k l).
+
+  Definition coerce(k1 k2:A.key_t)(H:k1 = k2)(v:A.value_t k1) : A.value_t k2.
+    intros. rewrite H in v. apply v.
+  Defined.
+
+  Ltac uncoerce :=
+    let rev_hyps := repeat 
+      match goal with
+        | [H: _ = _ |- _ ] => 
+          match goal with
+            | [H2: context [H]|- _ ] => revert H2
+          end 
+      end 
+      in let gen_eqs := repeat 
+        match goal with
+          | [H: _ = _ |- _ ] => 
+            match goal with
+              | [|- context [H]] => generalize H
+            end 
+        end 
+        in let refl_eqs := repeat 
+          match goal with
+            [|- forall (x : ?a = ?a), _] => 
+            let H2 := (fresh "H") in 
+              intro H2; rewrite (key_eq_irr H2); clear H2
+          end in
+          rev_hyps; gen_eqs; subst; refl_eqs; simpl.
+
+  Fixpoint lookup(k:A.key_t)(l:alist_t) {struct l} : option(A.value_t k) := 
+    match l with
+    | nil => None
+    | (k',, v'):: l' => 
+      match k' =! k with
+      | left k_eq_k' => Some (coerce k_eq_k' v')
+      | right k_neq_k' => lookup k l'
+      end
+    end.
+
+    Fixpoint distinct (l:alist_t) : Prop :=
+      match l with
+        | nil => True
+        | (k,,v)::ls => lookup k ls = None /\ distinct ls
+      end.
+    
+    Ltac simpler := try uncoerce;
+      repeat (progress ((repeat 
+        match goal with
+        | [H:?e = ?e |- _] => clear H
+        | [H:?k = ?k |- _ ] =>
+          match goal with
+            [|- context [H]] =>  rewrite (key_eq_irr H); simpl
+          end
+        | [|- context [match ?k1 =! ?k2 with 
+                         | left _ => _ 
+                         | right _ => _ end]] =>
+        case_eq (k1 =! k2) ; intros; try congruence ; try solve [assert False; intuition]; try subst 
+        | [H:context [match ?k1 =! ?k2 with 
+                         | left _ => _ 
+                         | right _ => _ end] |- _] =>
+        destruct (k1 =! k2) ; try congruence ; try solve [assert False; intuition]; try subst
+        |[H: sigT _ |- _] => destruct H
+        | [H: _ = _ |- context [coerce ?pf _]] => equate pf H || equate pf (sym_eq H)
+        | [H: _ = _ |- _ ] =>
+          match goal with
+            [|- context [H]] => let H2 := (fresh "H") in 
+              progress (generalize H; rewrite H; intro H2; rewrite (key_eq_irr H2); clear H2; simpl)
+          end
+        | [H: ?a = ?b |- _] => subst b || subst a
+      end); simpl in *; auto)).
+
+  (* interactions of lookup and the other operations *)
+  Lemma lookup_remove_eq k l : lookup k (remove k l) = None.
+  Proof. induction l; simpler. Qed.
+
+  Lemma lookup_remove_neq k k' l : k <> k' -> lookup k (remove k' l) = lookup k l.
+  Proof. induction l; simpler. Qed.
+
+  Lemma lookup_insert_eq k v l : lookup k (insert v l) = Some v.
+  Proof. induction l; simpler. Qed.
+
+  Lemma lookup_insert_neq k k' (v:value_t k') l : k <> k' -> lookup k (insert v l) = lookup k l.
+  Proof. induction l; simpler. Qed.
+
+  Lemma lookup_none_remove k l : lookup k l = None -> remove k l = l.
+  Proof. induction l; simpler. f_equal; auto. Qed.
+
+  Lemma lookup_none_perm k l l' : Permutation l l' -> lookup k l = None -> lookup k l' = None.
+  Proof. induction 1; simpler. Qed.
+
+  (* interactions of distinct and ther other operations *)
+  Lemma distinct_remove k l : distinct l -> distinct (remove k l).
+  Proof. induction l; simpler; intuition. rewrite lookup_remove_neq; auto. Qed.
+
+  Lemma distinct_insert k (v:A.value_t k) l : distinct l -> distinct (insert v l).
+  Proof. induction l; simpler; intuition. rewrite lookup_remove_neq; auto. Qed.
+
+  Lemma distinct_perm l l' : Permutation l l' -> distinct l -> distinct l'.
+  Proof. Hint Resolve lookup_none_perm. induction 1; simpler; intuition (congruence||eauto). Qed.
+
+  Hint Resolve lookup_remove_eq distinct_remove distinct_perm Permutation_sym Permutation_refl.
+
+  Lemma lookup_dis_perm k l l' : Permutation l l' -> distinct l -> lookup k l = lookup k l'.
+  Proof. induction 1; simpler; intuition try congruence. rewrite H2. eauto. Qed.
+
+  Lemma remove_perm k l l' : Permutation l l' -> Permutation (remove k l) (remove k l').
+  Proof.  Hint Constructors Permutation. induction 1; simpler; eauto. Qed.
+  Hint Resolve remove_perm.
+
+  Lemma insert_perm k l l' (v:A.value_t k) : Permutation l l' -> Permutation (insert v l) (insert v l').
+  Proof. unfold insert; simpler. Qed.
+  Hint Resolve insert_perm.
+
+  Lemma remove_swap k k' l : remove k (remove k' l) = remove k' (remove k l).
+  Proof. induction l; simpler. Qed.
+  Hint Resolve remove_swap.
+
+  Lemma insert_swap k (v:A.value_t k) k' (v':A.value_t k') l : k <> k' -> 
+    Permutation (insert v (insert v' l)) (insert v' (insert v l)).
+  Proof. intros. Hint Constructors Permutation. unfold insert; simpler. rewrite remove_swap. auto. Qed.
+  Hint Resolve insert_swap.
+
+End AssocList.
